# Week 5 - Power Series

[TOC]

## Definition

* A **power series** is a series of the form \\[\sum_{n=0}^{\infty}c_n x^n = c_0 + c_1 x + c_2 x^2 + c_3 x^3 + \cdots\\] where **x** is a variable and the \\(c_n\\)â€™s are constants called the **coefficients** of the series.
* The sum of the series is a function \\[f(x) = c_0 + c_1 x + c_2 x^2 + \cdots + c_n x^n + \cdots \\] whose domain is the set of all x for which the series converges. Notice that \\(f\\) resembles a polynomial.

## Convergence of Power Series

### Interval of convergence

* \\[C = \{ x \in \mathbb{R} | \sum_{n = 0}^{\infty} a_n x^n\ \text{converge}\}\\]
* **C** is called the **interval of convergence**.

### Theorem

* Suppose \\(\displaystyle \sum_{n = 0}^{\infty} a_n x^n\\) converge when \\(x = x_0\\), then the series converge absolutely x between \\(-x_0\\) and \\(x_0\\).

* Prove:
    * Suppose \\(\displaystyle \sum_{n = 0}^{\infty} a_n x^n\\) converge when \\(x = x_0\\)
    * So, \\(\lim_{n \to \infty} a_n x_o^n = 0\\),
    * There is an **M**, so that for all **n**, \\(|a_n x_0^n| \le M\\),
    * Pick \\(x \in (-|x_0|, |x_0|)\\),
    * \\(|a_n x^n| = |a_n x_0^n| \cdot |\frac{x^n}{x_0^n}| \le M \cdot |\frac{x^n}{x_0^n}|\\)
    * With ratio test, \\(r = |\frac{x^n}{x_0^n}| < 1\\), we can get \\(\sum_{n = 0}^{\infty} M \cdot r^n\\) converge,
    * So \\(\sum_{n=0}^{\infty} |a_n x^n|\\) converge.

* Corollary:
    * Consider \\(\sum_{n=0}^{\infty} a_n x^n\\).
    * There is an **R**, so that the series,
        * converges absolutely for \\(x \in (-R, R)\\),
        * diverges for \\(x > R \text{ or } x < -R\\)
    * The number **R** is called the **radius of convergence** of the power series.

### Example

* What's the interval of convergence of the series \\(\displaystyle \sum_{n=1}^{\infty}\frac{x^n}{n}\\)
* First, we ask the easier question. What's its radius of convergence?
    * Think this series converge absolutely, and use ratio test:
        * \\(\displaystyle\lim_{n \to \infty}|\frac{x^{n+1}/{n+1} }{x^n/n}| = |x|\\)
        * \\(|x|<1\\), the series converges,
        * \\(|x|>1\\), the series diverges.
    * So the radius of convergence is **1**.
* What about the endpoints **1** and **-1**?
    * if x = 1, then the series = \\(\sum_{n=1}^{\infty} \frac{1}{n}\\), which is harmonic series, also diverges.
    * if x = -1, then the series = \\(\sum_{n=1}^{\infty} \frac{(-1)^n}{n}\\), that's the alternating harmonic series, and converges.
* To summarize this: 
    * The interval of convergence of series \\(\displaystyle \sum_{n=1}^{\infty}\frac{x^n}{n}\\) is \\([-1, 1)\\)

## Differentiation and integration of power Series

### Power Series Centered Around a

* \\(\displaystyle\sum_{n=0}^{\infty}c_n (x - a)^n\\)
* Use ratio test:
    * \\(\displaystyle \lim_{n \to \infty} |\frac{C_{n+1} \cdot (x - a)^{n+1} }{C_n \cdot (x - a)^n}| = \lim_{n \to \infty} |\frac{C_{n+1} }{C_n}| \cdot |x - a|\\)
    * To get the interval of convergence, let's set \\(|\frac{C_{n+1} }{C_n}| = \frac{1}{R}\\)
        * \\(\frac{1}{R} \cdot |x - a| < 1\\)
        * \\(a - R < x < a + R\\)

### Differentiate a Power Series

* Theorem: 
    * \\(\displaystyle f(x) = \sum_{n=0}^{\infty} a_n x^n\\), **R** = radius of convergence.
    * Then \\(\displaystyle f'(x) = \sum_{n=1}^{\infty} n \cdot a_n \cdot x^{n-1} \text{ for } x \in (-R, R)\\)
        * Notice the index of **n** start from 1, because when \\(n = 0, f'(x) = 0\\)

### Integrate a Power Series

* Theorem: 
    * \\(\displaystyle f(x) = \sum_{n=0}^{\infty} a_n x^n\\), **R** = radius of convergence.
    * Then \\(\displaystyle \int_0^t f(x) dx = \sum_{n=1}^{\infty} \frac{a_n \cdot t^{n+1} }{n+1} \text{ for } x \in (-R, R)\\)
* Example: \\(\displaystyle \int_{x=0}^{t} \sum_{n=0}^{\infty} x^n dx\\)
    * First to prove: \\(\displaystyle \sum_{n=0}^{\infty} x^n = \frac{1}{1-x}\\), \\(|x| < 1\\) => \\(R = 1\\)
        * Use Geometric Series theorem, we know \\(\displaystyle \sum_{n=1}^{\infty} x^n = \sum_{n=1}^{\infty} x \cdot x^{n-1} = \frac{x}{1-x}\\)
        * So \\(\displaystyle \sum_{n=0}^{\infty} x^n = \frac{x}{1-x} + x^0 = \frac{1}{1-x}\\)
    * \\(\displaystyle \int_{x = 0}^t \frac{1}{1-x} dx\\), use substitution rule, set \\(u = 1 - x, du = -dx\\)
    * \\(\displaystyle \int_{x = 0}^t \frac{1}{1-x} dx = - \int_{x = 0}^t \frac{du}{u} \\)
    * \\(= -\log|u| \rbrack_{x=0}^t = - \log|1-x|\rbrack_{x=0}^t = - \log |1 - t|\\)
    * In another way, we can backwards the derivation:
        * \\(\displaystyle - \log |1 - t| = \int_{x=0}^t \frac{1}{1-x} dx\\)
        * \\(\displaystyle = \int_{x=0}^{t} \sum_{n=0}^{\infty} x^n dx = \sum_{n=0}^{\infty} \int_{x=0}^{t} x^n dx\\)
        * \\(\displaystyle = \sum_{n=0}^{\infty} \frac{t^{n+1} }{n+1}, |t| < 1\\)

### e^x

* To prove \\(\displaystyle \sum_{n=0}^{\infty} \frac{x^n}{n!} = e^x\\)
    *  It's the sum, n goes from 0 to infinity of x to the n over n factorial
* \\(\displaystyle f(x) = \sum_{n=0}^{\infty} \frac{x^n}{n!}\\)
* prove \\(f(0) = e^0 = 0\\):
    * \\(\displaystyle f(0) = \sum_{n=0}^{\infty} \frac{0^n}{n!} = 1\\)
        * \\(0^0 = 1, 0^1 = 0, \ldots, 0^n = 0\\)
        * \\(0! = 1\\). because: \\((n+1)! = (n+1) \cdot n!\\)
    * \\(e^0 = 1\\)
* after differentiation, both functions still themselves:
    * \\(\displaystyle \frac{d}{dx} \sum_{n=0}^{\infty} \frac{x^n}{n!} = \sum_{n=0}^{\infty} \frac{x^{n-1} }{(n-1)!} = \sum_{n=0}^{\infty} \frac{x^n}{n!} \\)
    * \\(\frac{d}{dx}e^x = e^x\\)
 *  These two star-crossed functions agree at a single point, and they're changing in the same way, and consequently, they must be the same function. 

### Multiply Two Power Series

* \\(\displaystyle (\sum_{n=0}^{\infty} a_n x^n) \cdot (\sum_{n=0}^{\infty} b_n x^n) \\)
* \\(=(a_0 + a_1 x + a_2 x^2 + \cdots) \cdot (b_0 + b_1 x + b_2 x^2 + \cdots)\\)
* \\(= a_0 b_0 + (a_1 + b_1) x + (a_0 b_2 + a_1 b_1 + a_2 b_0) x^2 + \cdots\\)
* \\(\displaystyle (\sum_{n=0}^{\infty} a_n x^n) \cdot (\sum_{n=0}^{\infty} b_n x^n) = \sum_{n=0}^{\infty} (\sum_{i=0}^{n} a_i b_{n-i}) x^n\\)

#### Theorem

* \\(f(x) = \displaystyle (\sum_{n=0}^{\infty} a_n x^n)\\), \\(g(x) = \displaystyle (\sum_{n=0}^{\infty} b_n x^n)\\), and their radius of convergence \\(\ge \mathbb{R}\\)
* Then we can get: \\(\displaystyle f(x) g(x) = \sum_{n=0}^{\infty} (\sum_{i=0}^{n} a_i b_{n-i}) x^n\\), for \\(x \in (-R, R)\\)

* Example: 
    * \\(\displaystyle e^x = \sum_{n=0}^{\infty} \frac{x^n}{n!} = 1 + x + \frac{x^2}{2} + \frac{x^3}{6} + \cdots \\)
    * \\((e^x)^2 = e^{(2x)}\\)
    * \\(e^{(2x)} = 1 + 2x + 2x^2 + \frac{8x^3}{6} + \cdots \\)
    * \\((e^x)^2 = (1 + x + \frac{x^2}{2} + \frac{x^3}{6} + \cdots)^2 \\)
        * \\(= 1 + 2x + (\frac{1}{2} + 1 + \frac{1}{2}) x^2 + (\frac{1}{6} + \frac{1}{2} + \frac{1}{2} + \frac{1}{6}) x^3 + \cdots\\)

## Fibonacci Numbers

### Transform 1/(1-x)

* \\(\displaystyle \sum_{n=0}^{\infty} x^n = \frac{1}{1-x}\\)
* Two ways to transfer \\(\frac{1}{(1-x)^2}\\)
    * First:
        * \\(\displaystyle \frac{1}{(1-x)^2} = \frac{d}{dx} (\frac{1}{1-x}) = \frac{d}{dx} \sum_{n=0}^{\infty} x^n = \sum_{n=0}^{\infty} \frac{d}{dx}(x^n) = \sum_{n=1}^{\infty} n \cdot x^{n-1}\\)
        * \\(= 1 \cdot x^0 + 2 \cdot x^1 + 3 \cdot x^2 + \cdots \\)
        * \\(\displaystyle = \sum_{n=0}^{\infty} (n+1) \cdot x^n\\)
    * Second:
        * \\(\displaystyle (\sum_{n=0}^{\infty} x^n)^2 = (1+x+x^2+x^3+\cdots)(1+x+x^2+x^3+\cdots) \\)
        * \\(= 1 + 2x + 3x^2 + 4x^3 + \cdots\\)
        * \\(\displaystyle = \sum_{n=0}^{\infty} (n+1) \cdot x^n\\)
        * Or we can use the theorem of **Multiply Two Power Series** 
            * \\(\displaystyle \sum_{n=0}^{\infty} (\sum_{i=0}^{n} a_i b_{n-i}) x^n\\)
            * In this case, \\(a_i = b_{n-i} = 1\\),
            * So  \\(\displaystyle = \sum_{n=0}^{\infty} (\sum_{i=0}^{n} 1) x^n = \sum_{n=0}^{\infty} (n+1) \cdot x^n\\)

### A Formula for the Fibonacci Numbers

* Let's say, \\({a_n}\\) is Fibonacci Sequence, and \\(f(x) = \displaystyle \sum_{n=0}^{\infty} a_n x^n\\)
    * \\( = x + x^2 + 2x^3 + 3x^4 + 5x^5 + \cdots\\)
* Then:
    * \\( x \cdot f(x) = x^2 + x^3 + 2x^4 + 3x^5 + 5x^6 + \cdots\\)
    * \\( x^2 \cdot f(x) = x^3 + x^4 + 2x^5 + 3x^6 + 5x^7 + \cdots\\)  
* Conclude above equations, we get:
    * \\(f(x) - x \cdot f(x) - x^2 \cdot f(x) = x\\)
* So \\(\displaystyle f(x) = \frac{x}{1-x-x^2}\\)
* set \\(\displaystyle \phi = \frac{1+\sqrt{5} }{2}\\), after some calculation we get:
* \\[\begin{aligned} 
    f(x) &= \frac{1/{\sqrt{5} } }{1-(x \cdot \phi)} + \frac{-1/{\sqrt{5} } }{1-(x \cdot (1-\phi))} \\
    &= \frac{1}{\sqrt{5} } \cdot \frac{1}{1-(x \cdot \phi)} + \frac{-1}{\sqrt{5} } \cdot \frac{1}{1-(x \cdot (1-\phi))} \\
    &= \frac{1}{\sqrt{5} } \sum_{n=0}^{\infty} (x \cdot \phi)^n + \frac{-1}{\sqrt{5} } \sum_{n=0}^{\infty} (x \cdot (1 - \phi))^n \\
    &= \sum_{n=0}^{\infty} (\frac{1}{\sqrt{ 5 } } \cdot \phi^{n} - \frac{1}{\sqrt{ 5 } } \cdot (1 - \phi)^{n}) x^n \\
    &= \sum_{n=0}^{\infty} \frac{\phi^n - (1 - \phi)^n}{\sqrt{5} } x^n = \sum_{n=0}^{\infty} a_n x^n
    \end{aligned}\\]
* So, \\(\displaystyle a_n = \frac{\phi^n - (1 - \phi)^n}{\sqrt{5} } \\)

