# Week 6 - Gaussian Elimination

\[TOC\]

## Gaussian Elimination

* To solv the linear system: \\[\begin{array}{c c c c c c}

    2 \chi\_0 & + & 4 \chi\_1 & - & 2 \chi\_2 & = & -10 \

    4 \chi\_0 & - & 2 \chi\_1 & + & 6 \chi\_2 & = & 20 \

    6 \chi\_0 & - & 4 \chi\_1 & + & 2 \chi\_2 & = & 18

    \end{array}\\]

### Procedures

* **Transform linear system of equations to an upper triangular system**
  * Subtract \\(\lambda\_{1,0} = \(\color{blue}{4} / \color{red}{2} \) = 2\\) times the first equation from the second equation: \\[\begin{array}{c \| c} \text{Before} & \text{After} \ \begin{array}{c c c c c c} \color{red}{2} \chi\_0 & + & 4 \chi\_1 & - & 2 \chi\_2 & = & -10 \ 4 \chi\_0 & - & 2 \chi\_1 & + & 6 \chi\_2 & = & 20 \ 6 \chi\_0 & - & 4 \chi\_1 & + & 2 \chi\_2 & = & 18 \end{array} & \begin{array}{c c c c c c} 2 \chi\_0 & + & 4 \chi\_1 & - & 2 \chi\_2 & = & -10 \ & - & 10 \chi\_1 & + & 10 \chi\_2 & = & 40 \ 6 \chi\_0 & - & 4 \chi\_1 & + & 2 \chi\_2 & = & 18 \end{array} \end{array}\\]
  * Subtract \\(\lambda\_{2,0} = \( \color{blue}{6} / \color{red}{2} \) = 3\\) times the first equation from the third equation: \\[\begin{array}{c \| c} \text{Before} & \text{After} \ \begin{array}{c c c c c c} \color{red}{2} \chi\_0 & + & 4 \chi\_1 & - & 2 \chi\_2 & = & -10 \ & - & 10 \chi\_1 & + & 10 \chi\_2 & = & 40 \ \color{blue}{6} \chi\_0 & - & 4 \chi\_1 & + & 2 \chi\_2 & = & 18 \end{array} & \begin{array}{c c c c c c} 2 \chi\_0 & + & 4 \chi\_1 & - & 2 \chi\_2 & = & -10 \ & - & 10 \chi\_1 & + & 10 \chi\_2 & = & 40 \ & - & 16 \chi\_1 & + & 8 \chi\_2 & = & 48 \end{array} \end{array}\\]
  * Subtract \\(\lambda\_{2,0} = \( \color{blue}{-16} / \color{red}{-10} \) = 1.6\\) times the second equation from the third equation: \\[\begin{array}{c \| c} \text{Before} & \text{After} \ \begin{array}{c c c c c c} 2 \chi\_0 & + & 4 \chi\_1 & - & 2 \chi\_2 & = & -10 \ & \color{red}{-} & \color{red}{10 \chi\_1} & + & 10 \chi\_2 & = & 40 \ & \color{red}{-} & \color{red}{16 \chi\_1} & + & 8 \chi\_2 & = & 48 \end{array} & \begin{array}{c c c c c c} 2 \chi\_0 & + & 4 \chi\_1 & - & 2 \chi\_2 & = & -10 \ & - & 10 \chi\_1 & + & 10 \chi\_2 & = & 40 \ & & & - & 8 \chi\_2 & = & - 16 \end{array} \end{array}\\]
  * This now leaves us with an upper triangular system of linear equations.
* **Back substitution \(solve the upper triangular system\)**
  * The equivalent upper triangular system of equations is now solved via back substitution:
    * Consider the last equation, \\[-8 \chi\_2 = -16.\\] Scaling both sides by by 1/\(âˆ’8\) we find that \\[\chi\_2 = -16/\(-8\) = 2.\\]
    * Next, consider the second equation, \\[-10 \chi\_1 + 10 \chi\_2 = 40.\\] We know that \\(\chi\_2 = 2\\), which we plug into this equation to yield \\[-10\chi\_1 + 10\( \color{blue}{2} = 40.\)\\] Rearranging this we find that \\[\chi\_1 = \(40 - 10\( \color{blue}{2} \)\)/\(-10\) = -2.\\]
    * Finally, consider the first equation, \\[2\chi\_0 + 4\chi\_1 - 2\chi\_2 = -10 \\] We know that \\(\chi\_2 =  \color{blue}{2} \\) and \\(\chi\_1 = \color{blue}{-2} \\), which we plug into this equation to yield \\[2\chi\_0 + 4\( \color{blue}{-2} \) - 2\( \color{blue}{2} \) = -10.\\] Rearranging this we find that \\[\chi\_0 = \(-10 - \(4\( \color{blue}{-2} \) - \(2\)\( \color{blue}{2} \)\)\)/2 = 1.\\]
* Thus, the solution is vector \\[x = \left\(\begin{array}{c} \chi\_0 \ \chi\_1 \ \chi\_2 \end{array}\right\) = \left\(\begin{array}{c} 1 \ -2 \ 2 \end{array}\right\).\\]
* **Check your answer** \(by plugging \\(\chi\_0 = 1, \chi\_1 = -2, \text{and}  \chi\_2 = 2\\) into the original system\).

### Representing the system of equations with an appended matrix

* ![](../.gitbook/assets/15231973476841%20%281%29.jpg)

### Transform matrix to upper triangular matrix

* ![](../.gitbook/assets/15231974994600%20%281%29.jpg)
* **Forward substitution \(applying the transforms to the right-hand side\)**
* ![](../.gitbook/assets/15231975659888%20%281%29.jpg)

### Algorithms

* ![](../.gitbook/assets/15231979384284.jpg)
* ![](../.gitbook/assets/15231979559406.jpg)

## Solving Ax = b via LU Factorization

### LU Factorization

* A matrix \\(A \in R^{n \times n}\\) can be factored into the product of two matrices \\(L,U \in R^{n \times n}\\) : \\[A= LU\\] where L is unit lower triangular and U is upper triangular.
* LU Factorization is transfer A to a LU combined matrix.
  * We can do this, because L is unit lower triangle matrix and U is upper triangle matrix.
* ![](../.gitbook/assets/15231982087014.jpg)
* ![](../.gitbook/assets/15231982335804.jpg)
* After rearrange, we get:
  * ![](../.gitbook/assets/15231983143005%20%281%29.jpg)
* Partition matrix A:
  * Update \\(a_{21} = a_{21}/ \alpha_{11} \(= l_{21}\)\\)
  * Update \\(A_{22} = A_{22} - a_{21} a_{12}^T\\) \(Rank-1 update!\)
  * Overwrite \\(A_{22}\\) with \\(L_{22}\\) and \\(U_{22}\\) by repeating with \\(A = A_{22}\\).
* This will leave U in the upper triangular part of A and the strictly lower triangular part of L in the strictly lower triangular part of A. The diagonal elements of L need not be stored, since they are known to equal one.

#### Algorithm

* ![](../.gitbook/assets/15231985740688%20%281%29.jpg)

### Where is this going?

1. Want to solve: \\(Ax = b\\)
   * Give A and b, solve x.
   * \\[A = \left\(\begin{array}{c c c}

     2 & + 4 & - 2 \

     4 & - 2 & + 6 \

     6 & - 4 & + 2

     \end{array}\right\), 

     b = \left\(\begin{array}{c}

     -10 \ 20 \ 18

     \end{array}\right\)\\]
2. Now we find triangular L and U so that: \\(A = LU\\)
   * U is the transformed A matrix
   * A is the coefficients which transfers A to U
   * Transfered: \\[A \to \left\(\begin{array}{c c c}

     2 & + 4 & - 2 \

     \scriptsize{2} & - 10 & - 10 \

     \scriptsize{3} & \scriptsize{1.6} & - 8

     \end{array}\right\),

     L = \left\(\begin{array}{c c c}

     1 & 0 & 0 \

     2 & 1 & 0 \

     3 & 1.6 & 1

     \end{array}\right\),

     U = \left\(\begin{array}{c c c}

     2 & + 4 & - 2 \

     0 & - 10 & + 10 \

     0 & 0 & - 8

     \end{array}\right\)\\]
3. Substitute: \\(\(LU\)x = b\\) =&gt; \\(L\(Ux\) = b\\)
4. Replace Ux with y. \(\\(y = Ux\\)\) =&gt; \\(Ly = b\\)
5. Solve \\(Ly = b\\) for \\(y\\). \(**More details in next section**\)
   * This is forward substitution \(applying the transforms to the right-hand side\).
   * \\[\left\(\begin{array}{c c c}

     1 & 0 & 0 \

     2 & 1 & 0 \

     3 & 1.6 & 1

     \end{array}\right\) \times 

     \left\(\begin{array}{c} 

     y\_0 \ y\_1 \ y\_2

     \end{array}\right\) =

     \left\(\begin{array}{c}

     -10 \ 20 \ 18

     \end{array}\right\) \\]

   * \\[\to \left\(\begin{array}{c}

       -10 \

       20 - 2 y\_0 \ 

       18 - 3 y\_0

     \end{array}\right\) \to \left\(\begin{array}{c}

       -10 \

       40 \ 

       48 - 1.6 y\_1

     \end{array}\right\) \to \left\(\begin{array}{c}

       -10 \

       40 \ 

       -16

     \end{array}\right\)\\]
6. Solve \\(Ux = y\\) for \\(x\\). \(**More details in next next section**\)
   * This is back substitution \(solve x\).
   * \\[\left\(\begin{array}{c c c}

     2 & + 4 & - 2 \

     0 & - 10 & + 10 \

     0 & 0 & - 8

     \end{array}\right\) \times 

     \left\(\begin{array}{c} 

     x\_0 \ x\_1 \ x\_2

     \end{array}\right\) = \left\(\begin{array}{c}

       -10 \ 40 \  -16

     \end{array}\right\) \\]

   * \\[ \to \left\(\begin{array}{c}

       -10 \ 40 \  \frac{-16}{-8} = \color{blue}{2}

     \end{array}\right\) \to \left\(\begin{array}{c} - 10 \

       \frac{40 - 10 \times \color{blue}{2} }{-10} = \color{red}{- 2} \ 

       \color{blue}{2}

     \end{array}\right\) \to \left\(\begin{array}{c}

       \frac{-10 - 4 \times \( \color{red}{- 2} \) - \( -2 \) \times \color{blue}{2}}{2} = \color{green}{1} \ \color{red}{- 2} \ \color{blue}{2}

     \end{array}\right\) \to \left\(\begin{array}{c}

       \color{green}{1} \ \color{red}{- 2} \ \color{blue}{2}

     \end{array}\right\)\\]

### Solving Lz = b \(Forward substitution\)

* Given a unit lower triangular matrix \\(L \in \mathbb{R}^{n \times n}\\) and vectors \\(z, b \in \mathbb{R}^{n}\\) , consider the equation \\(Lz = b\\) where L and b are known and z is to be computed. Partition
* ![](../.gitbook/assets/15232550852200.jpg)
* So, solving \\(Lz = b\\), overwriting b with z, is forward substitution when L is the unit lower triangular matrix that results from LU factorization.

#### Algorithm

* Algorithm for solving Lx = b, overwriting b with the result vector x. Here L is a lower triangular matrix.
* ![](../.gitbook/assets/15231996544107.jpg)

### Solving Ux = b \(Back substitution\)

* ![](../.gitbook/assets/15232553109209.jpg)

#### Algorithm

* ![](../.gitbook/assets/15231996940363.jpg)

### Cost

* Factoring \\(A = LU\\) requires, approximately, \\(\frac{2}{3}n^3\\) floating point operations.
* Solve \\(Lz = b\\) requires, approximately, \\(n^2\\) floating point operations.
* Solve \\(Ux = z\\) requires, approximately, \\(n^2\\) floating point operations.

